uml: Implement lean encoder part 7

plugins/Types/UML/edu.toronto.cs.se.mmint.types.uml.operators/lean/Architectural/ArchWithContracts.lean
@@ -2,6 +2,11 @@ import Architectural.Architecture
 import Architectural.Map
 variables {Var : Type} [fintype Var] [decidable_eq Var] 
 
+meta def auto_all_comps : tactic unit :=
+   `[ simp,
+    repeat {all_goals {split}},
+    repeat {exact with_top.coe_ne_top,}]
+
 structure ArchitectureWithContracts  (Φ : Type)  [AssertionLang Φ Var] (S : Component Var) extends Architecture S := 
 (parent : Contract Φ Var)
 (contracts : Map (Component Var) (Contract Φ Var))
@@ -10,14 +15,3 @@ structure ArchitectureWithContracts  (Φ : Type)  [AssertionLang Φ Var] (S : Co
 instance {Φ : Type} [AssertionLang Φ Var]  {S : Component Var} : has_coe (ArchitectureWithContracts Φ S) (Architecture S)  := 
 { coe := λ A , { ..A} }
 
-
--- def Construct 
--- (Φ : Type)  [AssertionLang Φ Var] 
--- (S : Component Var)
--- (SC : Contract Φ Var)
--- (A : Architecture S)
--- (contracts : Map (Component Var) (Contract Φ Var))
--- (all_components : ∀ S ∈ A.subs, contracts.find_val S ≠ none) : 
-
--- ArchitectureWithContracts Φ ⟨S,SC⟩ 
---  := ArchitectureWithContracts.mk {subs := A.subs} contracts all_components
